backends/lean/Aeneas/SLPoC/Tests/Examples/Basic.lean
@@ -1,4 +1,4 @@
-import Aeneas.SLPoC.RustHeap
+import Aeneas.SLPoC.MutableData.Ptr
 
 namespace Aeneas.SLPoC
 
